proof/BigNum_instances.ec
@@ -1,0 +1,23 @@
+from Jasmin require import JBigNum.
+
+require Array32 Array64 Array128 Array3.
+
+abbrev nlimbs = 32.
+abbrev dnlimbs = 64.
+
+clone import BigNum as W64xN with
+ op nlimbs <- nlimbs,
+ theory R.A <= Array32.Array32,
+ theory R2.A <= Array64.Array64,
+ theory Array3 <= Array3.Array3
+proof*.
+realize gt0_nlimbs by done.
+
+
+clone import BigNum as W64x2N with
+ op nlimbs <- dnlimbs,
+ theory R.A <= Array64.Array64,
+ theory R2.A <= Array128.Array128,
+ theory Array3 <= Array3
+proof*.
+realize gt0_nlimbs by done.
